custom mutex proof mostly done
Fix invariant.
Add specs for all functions in MyMutex.
Not sure if we need do_store_C or do_load_C.

rocq-brick-libstdcpp/test/mutex/custom_mutex.hpp
@@ -37,6 +37,8 @@ class MyMutex {
   }
 public:
 
+  MyMutex() {}
+
   void lock() {
     std::thread::id this_id{std::this_thread::get_id()};
 
