rocq-brick-libstdcpp/test/mutex/custom_mutex_hpp_proof.v
@@ -1,26 +1,121 @@
 (** Provisional *)
 
+Require Import iris.algebra.lib.excl_auth.
+Require Import iris.algebra.gset.
+
 Require Import skylabs.auto.cpp.proof.
+Require Import skylabs.auto.cpp.hints.base_derived.
 Require Import skylabs.brick.libstdcpp.mutex.spec.mutex.
+Require Import skylabs.brick.libstdcpp.mutex.requirements.
 Require Import skylabs.brick.libstdcpp.lib.lock_ghost.
 Require Import skylabs.brick.libstdcpp.atomic.spec.
+Require Import skylabs.brick.libstdcpp.cassert.spec.
 
 Require Import skylabs.brick.libstdcpp.test.mutex.custom_mutex_hpp.
 
 Module custom_mutex.
 
+  #[local] Existing Instance lock_ghost.has_lock.
+  #[local] Existing Instance lock_ghost.has_lock_upd.
+  #[local] Existing Instance lock_ghost.has_lock_valid.
+
   Abbreviation N := "MyMutex"%cpp_name.
 
-
+  (* FIXME maybe don't need to split it? *)
   Parameter thread_idR : ∀ `{Σ : cpp_logic, σ : genv}, cQp.t ->
     (* None if value is thread::id(), Some otherwise *)
     option thread_idT -> Rep.
-  #[only(timeless)] derive thread_idR.
+  #[only(cfracsplittable, type_ptr="std::thread::id")] derive thread_idR.
+  #[global] Axiom thread_idR_WeaklyObjective :
+    ∀ `{Σ : cpp_logic, σ : genv} (q : cQp.t)
+      (o : option thread_idT) (p : ptr),
+      WeaklyObjective (thread_idR q o p).
+  #[global] Existing Instance thread_idR_WeaklyObjective.
 
-  Parameter owner_token_auth : ∀ `{Σ : cpp_logic}, iprop.gname -> option thread_idT -> mpred.
-  Parameter owner_token_frac : ∀ `{Σ : cpp_logic}, iprop.gname -> option thread_idT -> mpred.
+  #[local] Instance at_WeaklyObjective `{Σ : cpp_logic}
+      (p : ptr) (R : Rep) `{!WeaklyObjective (R p)} :
+    WeaklyObjective (p |-> R).
+  Proof. rewrite INTERNAL._at_eq. apply _. Qed.
+
+  Canonical Structure owner_stateO := optionO thread_idTO.
+  Canonical Structure owner_tokenR := excl_authR owner_stateO.
+
+  Class ownerG `{Σ : cpp_logic} := {
+    #[local] has_owner_token :: HasOwn (iPropI _Σ) owner_tokenR;
+    #[local] has_owner_token_upd :: HasOwnUpd (iPropI _Σ) owner_tokenR;
+    #[local] has_owner_token_valid :: HasOwnValid (iPropI _Σ) owner_tokenR;
+  }.
+  #[global] Arguments ownerG {_ _} Σ : assert.
+
+  sl.lock
+  Definition owner_token_auth `{Σ : cpp_logic, !ownerG Σ}
+      (γ : iprop.gname) (o_thr : option thread_idT) : mpred :=
+    own γ (●E o_thr).
+  sl.lock
+  Definition owner_token_frac `{Σ : cpp_logic, !ownerG Σ}
+      (γ : iprop.gname) (o_thr : option thread_idT) : mpred :=
+    own γ (◯E o_thr).
   #[only(timeless, exclusive)] derive owner_token_auth.
   #[only(timeless, exclusive)] derive owner_token_frac.
+
+  #[global] Instance owner_token_auth_WeaklyObjective
+      `{Σ : cpp_logic, !ownerG Σ} γ o_thr :
+    WeaklyObjective (PROP := iPropI _) (owner_token_auth γ o_thr).
+  Proof. rewrite owner_token_auth.unlock. apply _. Qed.
+
+  #[global] Instance owner_token_frac_WeaklyObjective
+      `{Σ : cpp_logic, !ownerG Σ} γ o_thr :
+    WeaklyObjective (PROP := iPropI _) (owner_token_frac γ o_thr).
+  Proof. rewrite owner_token_frac.unlock. apply _. Qed.
+
+  Lemma owner_token_agree `{Σ : cpp_logic, !ownerG Σ}
+      γ (o1 o2 : option thread_idT) :
+    owner_token_auth γ o1 ** owner_token_frac γ o2 |-- [| o1 = o2 |].
+  Proof.
+    rewrite owner_token_auth.unlock owner_token_frac.unlock.
+    iIntros "[A F]".
+    iDestruct (own_valid_2 with "A F") as %HV.
+    iPureIntro.
+    apply leibniz_equiv, excl_auth_agree, HV.
+  Qed.
+
+  #[global] Instance owner_token_agree_observe
+      `{Σ : cpp_logic, !ownerG Σ} γ (o1 o2 : option thread_idT) :
+    Observe2 [| o1 = o2 |]
+      (owner_token_auth γ o1) (owner_token_frac γ o2).
+  Proof.
+    apply observe_2_intro_only_provable.
+    rewrite owner_token_auth.unlock owner_token_frac.unlock.
+    iIntros "A F".
+    iDestruct (own_valid_2 with "A F") as %HV.
+    iPureIntro.
+    apply leibniz_equiv, excl_auth_agree, HV.
+  Qed.
+
+  #[global] Instance owner_token_agree_observe_sep
+      `{Σ : cpp_logic, !ownerG Σ} γ (o1 o2 : option thread_idT) :
+    Observe [| o1 = o2 |]
+      (owner_token_auth γ o1 ** owner_token_frac γ o2).
+  Proof.
+    apply observe_intro_only_provable.
+    rewrite owner_token_auth.unlock owner_token_frac.unlock.
+    iIntros "[A F]".
+    iDestruct (own_valid_2 with "A F") as %HV.
+    iPureIntro.
+    apply leibniz_equiv, excl_auth_agree, HV.
+  Qed.
+
+  Lemma owner_token_update `{Σ : cpp_logic, !ownerG Σ}
+      γ (oa ofrag o' : option thread_idT) :
+    owner_token_auth γ oa ** owner_token_frac γ ofrag |--
+      (|==> owner_token_auth γ o' ** owner_token_frac γ o').
+  Proof.
+    rewrite owner_token_auth.unlock owner_token_frac.unlock.
+    iIntros "[A F]".
+    iMod (own_update_2 with "A F") as "[$ $]";
+      first apply (excl_auth_update _ _ o').
+    done.
+  Qed.
 
   Record gname : Set := MkGname
   { user_gname : iprop.gname
@@ -30,7 +125,8 @@ Module custom_mutex.
 
   Definition lock_namespace : namespace := nroot .@@ "MyMutex".
 
-  Definition locked `{Σ : cpp_logic} `{!lockG Σ} `{σ : genv}
+  sl.lock
+  Definition locked `{Σ : cpp_logic} `{!lockG Σ, !ownerG Σ} `{σ : genv}
       (γ: gname) (o_thr : option thread_idT) : Rep :=
     _field "MyMutex::m_owner" |-> thread_idR 1$m o_thr ** pureR (owner_token_frac γ.(phys_state_gname) o_thr).
   #[only(timeless, exclusive)] derive locked.
@@ -43,7 +139,11 @@ Module custom_mutex.
       _field "MyRecursiveMutex::m_count" |-> ulonglongR 1$m count. *)
 
   Section with_Σ.
-    Context `{Σ : cpp_logic, σ : genv, HAS_THREADS : !HasStdThreads Σ, !lockG Σ}.
+    Context `{Σ : cpp_logic, σ : genv, HAS_THREADS : !HasStdThreads Σ,
+      !lockG Σ, !ownerG Σ}.
+
+    (* Abbreviation BASE p :=
+      (p ,, _base "std::atomic<int>" "std::__atomic_base<int>"). *)
 
     Definition mutex_content (γ : gname) : Rep :=
       ∃ o_owner lockedb,
@@ -52,7 +152,8 @@ Module custom_mutex.
 
     Definition mutex_inv (this : ptr) (γ : gname) (P : mpred) : mpred :=
       ∃ b : bool,
-      this ,, _field "MyMutex::m_lock" |-> atomic.R "int" 1$m (if b then 1 else 0)%Z **
+      this ,, _field "MyMutex::m_lock" |->
+        atomic.R "int" 1$m (if b then 1 else 0)%Z **
       ∃ o_owner : option thread_idT,
       owner_token_auth γ.(phys_state_gname) o_owner **
       (if b then
@@ -78,35 +179,117 @@ Module custom_mutex.
 
     Context `{MOD : source ⊧ σ}.
 
+    Abbreviation GLOBALS q :=
+      (_global "std::memory_order_seq_cst" |->
+        primR "enum std::memory_order" q
+          (memory_order.to_val memory_order.seq_cst)).
+
+    cpp.spec (default_ctor "std::thread::id") as thread_id_ctor_spec with (
+      \this this
+      \post this |-> thread_idR 1$m None).
+
+    cpp.spec (const_copy_ctor "std::thread::id") as thread_id_copy_ctor_spec with (
+      \this this
+      \arg{other} "" (Vptr other)
+      \prepost{q o} other |-> thread_idR q o
+      \post this |-> thread_idR 1$m o).
+
+    cpp.spec (dtor "std::thread::id") as thread_id_dtor_spec with (
+      \this this
+      \pre{o} this |-> thread_idR 1$m o
+      \post emp).
+
+    cpp.spec "std::thread::id::operator=(const std::thread::id&)"
+        as thread_id_copy_assign_spec with (
+      \this this
+      \arg{other} "" (Vptr other)
+      \pre{old} this |-> thread_idR 1$m old
+      \prepost{q o} other |-> thread_idR q o
+      \post[Vref this] this |-> thread_idR 1$m o).
+
+    cpp.spec "std::thread::id::operator=(std::thread::id&&)"
+        as thread_id_move_assign_spec with (
+      \this this
+      \arg{other} "" (Vptr other)
+      \pre{old} this |-> thread_idR 1$m old
+      \prepost{o} other |-> thread_idR 1$m o
+      \post[Vref this] this |-> thread_idR 1$m o).
+
+    cpp.spec "std::operator==(std::thread::id, std::thread::id)"
+        as thread_id_eq_spec with (
+      \arg{lhs} "" (Vptr lhs)
+      \arg{rhs} "" (Vptr rhs)
+      \prepost{q1 o1} lhs |-> thread_idR q1 o1
+      \prepost{q2 o2} rhs |-> thread_idR q2 o2
+      \post[Vbool (bool_decide (o1 = o2))] emp).
+
+    cpp.spec "std::this_thread::get_id()" as get_id_spec with (
+      \persist{thr} current_thread thr
+      \post{result}[Vptr result]
+        result |-> thread_idR 1$m (Some thr)).
+
     cpp.spec "MyMutex::MyMutex()" as ctor_spec with (
       \this this
       \pre{P} ▷P
-      \post Exists g, this |-> IR g 1$m P ** used_threads g.(user_gname) ∅).
+      \require WeaklyObjective P
+      \post (|={⊤}=> Exists g,
+        this |-> IR g 1$m P ** used_threads g.(user_gname) ∅)).
 
     cpp.spec "MyMutex::~MyMutex()" as dtor_spec with (
       \this this
       \pre{g P} this |-> IR g 1$m P ** used_threads g.(user_gname) ∅
       \post P).
 
-    cpp.spec "MyMutex::do_lock()" as lock_spec with (
+    cpp.spec "MyMutex::do_lock()" as do_lock_spec with (
       \this this
       \prepost{q P g} this |-> IR g q P
       \persist{thr} current_thread thr
       \pre user g.(user_gname) thr
-      \prepost{q'} _global "std::memory_order_seq_cst" |-> primR "enum std::memory_order" q' (memory_order.to_val memory_order.seq_cst)
-      \post (▷ P **
+      \prepost{q'} GLOBALS q'
+      \post (P **
             this ,, _field "MyMutex::m_owner" |-> thread_idR 1$m None) **
             owner_token_frac g.(phys_state_gname) (Some thr)).
 
-    cpp.spec "MyMutex::do_unlock()" as unlock_spec with (
+    cpp.spec "MyMutex::do_unlock()" as do_unlock_spec with (
       \this this
       \prepost{q P g} this |-> IR g q P
       \persist{thr} current_thread thr
-      \pre ▷P
-      \pre this |-> locked g (Some thr)
+      \pre (▷P **
+            this ,, _field "MyMutex::m_owner" |-> thread_idR 1$m None) **
+            owner_token_frac g.(phys_state_gname) (Some thr)
       \post user g.(user_gname) thr).
 
-    (* Axiom *)
+    Definition T : Type := gname * mpred.
+
+    (* FIXME should GLOBALS be in lock specs, instead of do_lock? *)
+    Definition do_lock (this : ptr) (lk : T) (K : mpred) : mpred :=
+      let g := lk.1 in
+      let P := lk.2 in
+      ∃ thr q', current_thread thr ** user g.(user_gname) thr ** GLOBALS q' **
+        (GLOBALS q' ** P ** this |-> locked g (Some thr) -* K).
+    #[global] Arguments do_lock /.
+
+    Definition do_unlock (this : ptr) (lk : T) (K : mpred) : mpred :=
+      let g := lk.1 in
+      let P := lk.2 in
+      ∃ thr, current_thread thr ** this |-> locked g (Some thr) ** ▷P **
+        (user g.(user_gname) thr -* K).
+    #[global] Arguments do_unlock /.
+
+    #[global] Instance custom_mutex_basic_lockable :
+        BasicLockable (T := T) (Tnamed N)
+          (fun q gP => IR gP.1 q gP.2) :=
+      { do_lock := do_lock
+      ; do_unlock := do_unlock }.
+
+    cpp.spec "MyMutex::lock()" as lock_spec with
+      (\exact Reduce
+        (lock_basic_lockable (Tnamed N) (fun q gP => IR gP.1 q gP.2))).
+
+    cpp.spec "MyMutex::unlock()" as unlock_spec with
+      (\exact Reduce
+        (unlock_basic_lockable (Tnamed N) (fun q gP => IR gP.1 q gP.2))).
+
     cpp.spec "std::this_thread::yield()" as yield_spec with (
       \post emp).
 
@@ -142,68 +325,186 @@ Module custom_mutex.
       iDestruct (fupd_mask_subseteq) as ">Y"; [ | iModIntro ]; first solve_ndisj.
       work.
       1: admit. (* can and should be an AC *)
-      iMod "Y" as "_"; wpose "Hc"; work.
       wname [cinv] "CI".
       wname [owner_token_auth] "OA".
       wname [_ |-> atomic.R _ _ _] "FL".
       wname [_ |-> thread_idR _ _] "PF".
       wname [user _ _] "U".
       ren_hyp b bool.
-      destruct b eqn:?; work. {
-        iSplitL "OA FL PF"; first last. {
-          iModIntro. rewrite /IR/mutex_inv. work $usenamed=true.
-          auto.
-        }
-        work $usenamed=true with br_erefl.
-        iExists true, _.
-        ework $usenamed=true with br_erefl.
-      }
-      iDestruct "PF" as "(P & ? & OF)".
-      iSplitL "FL OA U"; first last. {
-        iModIntro. rewrite /IR/mutex_inv. ework $usenamed=true with br_erefl.
+      destruct b eqn:Hb.
+      - iMod "Y" as "_".
+        iMod ("Hc" with "[FL OA PF]") as "_".
+        { iNext. iExists true. iFrame. }
+        iModIntro. rewrite /IR. work $usenamed=true with br_erefl.
         auto.
-        (* perform ghost update, but earlier *)
-        admit.
-      }
-      work $usenamed=true with br_erefl.
-      iExists true, _.
-      ework $usenamed=true with br_erefl.
-      (* should be proved by the previously mentioned ghost update *)
-      admit. 
-      all: fail.
-
-      (* iSplitL "OG FO I FL"; first last. { *)
-      (*   iModIntro. rewrite /IR/mutex_inv. work $usenamed=true. *)
-      (*   wfocus [| _ |] "". { iPureIntro. destruct b; auto. } *)
-      (*   destruct b eqn:?; work. *)
-      (* } *)
-      (* destruct b eqn:?. { *)
-      (*   work $usenamed=true with br_erefl. *)
-      (*   iExists _, true. *)
-      (*   ework $usenamed=true with br_erefl. *)
-      (* } *)
-      (* work $usenamed=true with br_erefl. *)
-      (* iExists _, true. *)
-      (* ework $usenamed=true with br_erefl. *)
-      (* iApply affine; last iAccu. *)
+      - iDestruct "PF" as "(P & FO & OF)".
+        iMod (owner_token_update g.(phys_state_gname) _ _ (Some thr)
+          with "[$OA $OF]") as "(OA & OF)".
+        iMod "Y" as "_".
+        iMod ("Hc" with "[FL OA U]") as "_".
+        { iNext. iExists true. iFrame. done. }
+        iModIntro. rewrite /IR. work $usenamed=true with br_erefl.
+        auto.
     Admitted.
     Hint Resolve do_exchange_C : sl_opacity.
+
+    #[program]
+    Definition do_store_C (p : ptr) :=
+      \cancelx
+      \using denoteModule source
+      \using{thr} current_thread thr
+      \consuming{g q P} p |-> IR g q P
+      \consuming P
+      \consuming p ,, _field "MyMutex::m_owner" |-> thread_idR 1$m None
+      \consuming owner_token_frac g.(phys_state_gname) (Some thr)
+      \proving{K (_ : IsExistential K)}
+        std.atomic.do_store "int" (BASE (p ,, o_field σ "MyMutex::m_lock")) 0%Z K
+      \instantiate K := (p |-> IR g q P ** user g.(user_gname) thr)
+      \end@{mpredI}.
+    Next Obligation.
+      intros. iIntros "[#M ?]" (?? ->).
+      iDestruct (observe [| _ ⊧ _ |] with "M") as "%".
+      rewrite /std.atomic.do_store.
+      iAcIntro. rewrite /commit_acc /=.
+      rewrite {1}/IR/mutex_inv /=; work.
+      wname [cinv] "#?".
+      iInv lock_namespace as "?" "Hc"; work.
+      ren_hyp b bool.
+      iExists (if b then 1%Z else 0%Z). iFrame.
+      iApply fupd_mask_intro; first solve_ndisj.
+      iIntros "Y". iNext. iIntros "FL".
+      iMod "Y" as "_".
+      wname [P] "P".
+      wname [_ |-> thread_idR _ _] "FO".
+      wname [owner_token_frac] "OF".
+      wname [owner_token_auth] "OA".
+      iRename "P" into "CI".
+      wname [P] "RP".
+      wname [_ |-> thread_idR _ _] "OwnerField".
+      destruct b eqn:Hb.
+      - iDestruct "FO" as (owner) "(U & ->)".
+        iDestruct (observe [| Some owner = Some thr |]
+          (owner_token_auth g.(phys_state_gname) (Some owner) **
+           owner_token_frac g.(phys_state_gname) (Some thr))
+          with "[$OA $OF]")
+          as %Hagree.
+        inversion Hagree; subst owner.
+        iEval (rewrite _at_offsetR) in "FL".
+        iMod ("Hc" with "[FL OA RP OwnerField OF]") as "_".
+        { iNext. iExists false.
+          work $usenamed=true with br_erefl.
+          iExists (Some thr). iFrame. }
+        iModIntro. rewrite /IR. work $usenamed=true with br_erefl.
+      - iDestruct "FO" as "(RP2 & OwnerField2 & OF2)".
+        iEval (rewrite owner_token_frac.unlock) in "OF".
+        iEval (rewrite owner_token_frac.unlock) in "OF2".
+        iDestruct (own_valid_2 with "OF OF2") as %Hvalid.
+        rewrite excl_auth_frag_op_valid in Hvalid.
+        done.
+    Qed.
+    Hint Resolve do_store_C : sl_opacity.
+
+    #[program]
+    Definition do_load_C (p : ptr) :=
+      \cancelx
+      \using denoteModule source
+      \consuming{q (n : Z)} p |-> atomic.R "int" q n
+      \proving{(K : Z -> mpred) (_ : IsExistential K)}
+        std.atomic.do_load "int" (BASE p) K
+      \instantiate K :=
+        (fun x : Z => p |-> atomic.R "int" q n ** [| x = n |])
+      \end@{mpredI}.
+    Next Obligation.
+      intros. iIntros "[#M ?]" (?? ->).
+      iDestruct (observe [| _ ⊧ _ |] with "M") as "%".
+      rewrite /std.atomic.do_load.
+      iAcIntro. rewrite /commit_acc.
+      iDestruct (fupd_mask_subseteq) as ">Y"; [ | iModIntro ]; eauto.
+      work. iExists q. work.
+      iMod "Y". iModIntro.
+      work.
+    Qed.
+    Hint Resolve do_load_C : sl_opacity.
+
     Hint Opaque locked : sl_opacity.
 
-    Lemma test_do_lock_ok : verify[source] "MyMutex::do_lock()".
+    Lemma mymutex_do_lock_proof : verify[source] "MyMutex::do_lock()".
     Proof using MOD HAS_THREADS.
       verify_spec; go.
       wp_while (fun _ => emp); go; first by ework.
       wp_if; go.
     Qed.
 
-    Lemma test_do_unlock_ok : verify[source] "MyMutex::do_unlock()".
+    Lemma mymutex_do_unlock_proof : verify[source] "MyMutex::do_unlock()".
     Proof using MOD HAS_THREADS.
       verify_spec; go.
-      iExists (user g.(user_gname) thr).
-      rewrite /locked.
+    Qed.
+
+    Lemma mymutex_ctor_proof : verify[source] "MyMutex::MyMutex()".
+    Proof using MOD HAS_THREADS.
+      verify_spec; go.
+      wname [structR] "S".
+      iMod (own_alloc (● (GSet ∅ : lock_ghostUR))) as (gu) "UT".
+      { apply auth_auth_valid. done. }
+      iMod (own_alloc (●E None ⋅ ◯E None)) as (gp) "O".
+      { apply excl_auth_valid. }
+      iDestruct (own_op with "O") as "(OA & OF)".
+      iMod (cinv_alloc ⊤ lock_namespace
+        (mutex_inv this (MkGname gu gu gp) P) with "[-S UT]")
+        as (gi) "(#CI & CO)"; last first.
+      - iExists (MkGname gu gi gp).
+        rewrite /IR used_threads.unlock /=.
+        iModIntro. go $usenamed=true with br_erefl.
+      - rewrite /mutex_inv owner_token_auth.unlock
+          owner_token_frac.unlock /=.
+        iNext. iExists false. iFrame.
+    Qed.
+
+    Lemma mymutex_dtor_proof : verify[source] "MyMutex::~MyMutex()".
+    Proof using MOD HAS_THREADS.
+      verify_spec.
+      rewrite /IR /mutex_inv.
       work.
-    Admitted.
+      wname [cinv] "#CI".
+      wname [cinv_own] "CO".
+      iMod (cinv_cancel with "CI CO")
+        as "Inv"; [done..|].
+      go.
+      iDestruct "Inv" as (b) "(Lock & % & OA & State)".
+      destruct b eqn:Hb.
+      - iDestruct "State" as (th) "(U & %Eq)".
+        iDestruct (used_threads_empty_no_not_locked with "[$]") as %[].
+      - iDestruct "State" as "(P & Owner & OF)".
+        ego $usenamed=true with br_erefl.
+        wname [used_threads] "UT".
+        iApply (affine with "[OA OF UT]"); last iAccu. apply mpred_BiAffine.
+  Qed.
+
+    Lemma mymutex_lock_proof : verify[source] "MyMutex::lock()".
+    Proof using MOD HAS_THREADS.
+      verify_spec.
+      rewrite locked.unlock.
+      ego.
+    Qed.
+
+    Lemma mymutex_unlock_proof : verify[source] "MyMutex::unlock()".
+    Proof using MOD HAS_THREADS.
+      verify_spec.
+      rewrite locked.unlock.
+      go.
+      iExists _, _.
+      go.
+      iExists _, _, _, _.
+      go.
+      iExists _, _.
+      go.
+      iExists _, _.
+      go.
+      iExists _.
+      go.
+      iExists q, m.2, m.1.
+      go.
+    Qed.
 
 
   End with_Σ.
